\section*{Aufgabe 2}

Welche der folgenden aussagenlogischen Formeln sind Tautologien, welche sind erf√ºllbar?\\

\begin{itemize}[leftmargin=*]
\item \textit{Anmerkung:} $X \Rightarrow Y$ \textit{wurde hier als} $\lnot X \lor Y$ \textit{geschrieben}
\end{itemize}

a) $(A \Rightarrow (B \Rightarrow C)) \Leftrightarrow ((A \land B) \Rightarrow C)$\\


\begin{table}[h]
\centering
\begin{tabular}{c|c|c|c|c|c|c|c|c|c|c}
$A$ & $B$ & $C$ & $\lnot A$ & $\lnot B$ & $\overbrace{\lnot B \lor C}^{D}$ & $\overbrace{\lnot A \lor D}^{E}$ & $\overbrace{A \land B}^{F}$ & $\lnot F$ & $\overbrace{\lnot F \lor C}^{G}$ & $E \Leftrightarrow G$\\
\hline
1 & 1 & 1 & 0 & 0 & 1 & 1 & 1 & 0 & 1 & 1\\
1 & 0 & 1 & 0 & 1 & 1 & 1 & 0 & 1 & 1 & 1\\
0 & 1 & 1 & 1 & 0 & 1 & 1 & 0 & 1 & 1 & 1\\
0 & 0 & 1 & 1 & 1 & 1 & 1 & 0 & 1 & 1 & 1\\
1 & 1 & 0 & 0 & 0 & 0 & 0 & 1 & 0 & 0 & 1\\
1 & 0 & 0 & 0 & 1 & 1 & 1 & 0 & 1 & 1 & 1\\
0 & 1 & 0 & 1 & 0 & 0 & 1 & 0 & 1 & 1 & 1\\
0 & 0 & 0 & 1 & 1 & 1 & 1 & 0 & 1 & 1 & 1
\end{tabular}
\end{table}\

b) $((A \Rightarrow B) \Rightarrow C) \Leftrightarrow ((A \lor C) \land (\lnot B \lor C))$

\hspace{3.57cm}$\Leftrightarrow (C \lor (\lnot B \land A))$

\begin{table}[h]
\centering
\begin{tabular}{c|c|c|c|c|c|c|c|c|c|c|c}
$A$ & $B$ & $C$ & $\lnot A$ & $\lnot B$ & $\overbrace{\lnot A \lor B}^{D}$ & $\lnot D$ & $\overbrace{\lnot D \lor C}^{E}$ & $\overbrace{\lnot B \land A}^{F}$ & $\overbrace{C \lor F}^{G}$ & $E \Leftrightarrow G$\\
\hline
1 & 1 & 1 & 0 & 0 & 1 & 0 & 1 & 0 & 1 & 1\\
1 & 0 & 1 & 0 & 1 & 0 & 1 & 1 & 1 & 1 & 1\\
0 & 1 & 1 & 1 & 0 & 1 & 0 & 1 & 0 & 1 & 1\\
0 & 0 & 1 & 1 & 1 & 1 & 0 & 1 & 0 & 1 & 1\\
1 & 1 & 0 & 0 & 0 & 1 & 0 & 1 & 0 & 0 & 0\\
1 & 0 & 0 & 0 & 1 & 0 & 1 & 0 & 1 & 1 & 0\\
0 & 1 & 0 & 1 & 0 & 1 & 0 & 1 & 0 & 0 & 0\\
0 & 0 & 0 & 1 & 1 & 1 & 0 & 1 & 0 & 0 & 0\\
\end{tabular}
\end{table}\


c) $((A \Rightarrow B) \Rightarrow C) \Rightarrow (A \Rightarrow (B \land C))$\\

d) $((A \land \lnot B) \Rightarrow (A \lor C)) \Rightarrow (\lnot (B \Rightarrow A) \land (\lnot A \Rightarrow C))$\\

e) $(\lnot B \land A) \Leftrightarrow \lnot (A \Rightarrow B)$\\